Allow more things to move around! See msg.
Previously, we only allowed things to exchange amongst each other if
their rw-sets satisfied the following conditions: (1) their reads
don't coincide with the other's writes, and (2) their writes don't
coincide.

This is quite restrictive, since if two instructions were to perform a
write of a constant into a location, then it is actually safe to do
exchange them. With this commit, we can now check for this sort of
behavior and allow this sort of exchange.

In particular, we now check if two things have the exact same value
written. If they do so, then those values can be safely ignored when
comparing write-write set disjointness.

The concrete effect of this change is that now we are able to exchange
instructions that havoc the flags, as long as both instructions havoc
the flags.

---

This upgrade is a significant step forwards towards being able to
support the full level of instr-reordering which allows one to
exchange even entire blocks of code, even if individual instructions
themselves cannot be exchanged!

---

One MASSIVE caveat however is that this breaks our sanity-check for
instruction exchanges. In particular, if an instructions write values
are disjoint, it will disallow it due to non-same constant-write
values. To bring back the more forgiving behavior, it will require
examining and expanding the definition of [rw_exchange_allowed] to
allow more cases.

vale/code/lib/transformers/Vale.Transformers.InstructionReorder.fst
@@ -46,16 +46,36 @@ open Vale.Transformers.BoundedInstructionEffects
 
 module L = FStar.List.Tot
 
+/// Some convenience functions
+
+let rec locations_of_locations_with_values (lv:locations_with_values) : locations =
+  match lv with
+  | [] -> []
+  | (|l,v|) :: lv ->
+    l :: locations_of_locations_with_values lv
+
+let rec locations_subtract (a b:locations) : locations =
+  match a with
+  | [] -> []
+  | x :: xs ->
+    if List.Tot.mem x b then
+      locations_subtract xs b
+    else
+      x :: locations_subtract xs b
+
 /// Given two read/write sets corresponding to two neighboring
 /// instructions, we can say whether exchanging those two instructions
 /// should be allowed.
 
 let rw_exchange_allowed (rw1 rw2 : rw_set) : pbool =
-  let r1, w1 = rw1.loc_reads, rw1.loc_writes in
-  let r2, w2 = rw2.loc_reads, rw2.loc_writes in
+  let r1, w1, c1 = rw1.loc_reads, rw1.loc_writes, rw1.loc_constant_writes in
+  let r2, w2, c2 = rw2.loc_reads, rw2.loc_writes, rw2.loc_constant_writes in
+  let dw1 = w1 `locations_subtract` (locations_of_locations_with_values c1) in
+  let dw2 = w2 `locations_subtract` (locations_of_locations_with_values c2) in
+  ((c1 = c2) /- "writing different constants") &&.
   (disjoint_locations r1 w2 /+< "read set of 1st not disjoint from write set of 2nd because ") &&.
   (disjoint_locations r2 w1 /+< "read set of 2nd not disjoint from write set of 1st because ") &&.
-  (disjoint_locations w1 w2 /+< "write sets not disjoint because ")
+  (disjoint_locations dw1 dw2 /+< "dynamic write sets not disjoint because ")
 
 let ins_exchange_allowed (i1 i2 : ins) : pbool =
   (
@@ -72,19 +92,12 @@ let lemma_ins_exchange_allowed_symmetric (i1 i2 : ins) :
         !!(ins_exchange_allowed i1 i2)))
     (ensures (
         !!(ins_exchange_allowed i2 i1))) =
-  let b1 = !!(ins_exchange_allowed i1 i2) in
-  let b2 = !!(ins_exchange_allowed i2 i1) in
-  assert (b1 == !!(rw_exchange_allowed (rw_set_of_ins i1) (rw_set_of_ins i2)));
-  assert (b2 == !!(rw_exchange_allowed (rw_set_of_ins i2) (rw_set_of_ins i1)));
   let rw1, rw2 = rw_set_of_ins i1, rw_set_of_ins i2 in
-  let r1, w1 = rw1.loc_reads, rw1.loc_writes in
-  let r2, w2 = rw2.loc_reads, rw2.loc_writes in
-  let disjoint = disjoint_locations in
-  let aux l1 l2 : (b:bool) = !!(disjoint l1 l2) in
-  assert (b1 == (aux r1 w2 && aux r2 w1 && aux w1 w2));
-  assert (b2 == (aux r2 w1 && aux r1 w2 && aux w2 w1));
-  lemma_disjoint_locations_symmetric w1 w2;
-  assert (aux w1 w2 = aux w2 w1)
+  let r1, w1, c1 = rw1.loc_reads, rw1.loc_writes, rw1.loc_constant_writes in
+  let r2, w2, c2 = rw2.loc_reads, rw2.loc_writes, rw1.loc_constant_writes in
+  let dw1 = w1 `locations_subtract` (locations_of_locations_with_values c1) in
+  let dw2 = w2 `locations_subtract` (locations_of_locations_with_values c2) in
+  lemma_disjoint_locations_symmetric dw1 dw2
 
 /// First, we must define what it means for two states to be
 /// equivalent. Here, we basically say they must be exactly the same.
@@ -594,39 +607,83 @@ let rec lemma_unchanged_at_mem (as:list location) (a:location) (s1 s2:machine_st
     if a = x then () else
     lemma_unchanged_at_mem xs a s1 s2
 
-let lemma_unchanged_at_combine (a1 a2:list location) (sa1 sa2 sb1 sb2:machine_state) :
+let rec lemma_disjoint_locations_subtract (a a_ b:locations) :
+  Lemma
+    (requires (!!(disjoint_locations a b)))
+    (ensures (!!(disjoint_locations (a `locations_subtract` a_) b))) =
+  match a with
+  | [] -> ()
+  | x :: xs ->
+    lemma_disjoint_locations_subtract xs a_ b
+
+let rec lemma_disjoint_location_from_locations_subtract (a:location) (as as_:locations) :
   Lemma
     (requires (
-        !!(disjoint_locations a1 a2) /\
+        !!(disjoint_location_from_locations a (as `locations_subtract` as_)) /\
+        not (L.mem a as_)))
+    (ensures (!!(disjoint_location_from_locations a as))) =
+  match as with
+  | [] -> ()
+  | x :: xs -> lemma_disjoint_location_from_locations_subtract a xs as_
+
+let rec lemma_locations_subtract_mem (a:location) (as as_:locations) :
+  Lemma
+    (ensures (L.mem a (as `locations_subtract` as_) = (L.mem a as && not (L.mem a as_)))) =
+  match as with
+  | [] -> ()
+  | x :: xs ->
+    lemma_locations_subtract_mem a xs as_
+
+let lemma_unchanged_at_combine (a1 a2 a_:list location) (sa1 sa2 sb1 sb2:machine_state) :
+  Lemma
+    (requires (
+        !!(disjoint_locations (a1 `locations_subtract` a_) (a2 `locations_subtract` a_)) /\
+        (unchanged_at a_ sb1 sb2) /\
         (unchanged_at a1 sa1 sb2) /\
         (unchanged_except a2 sa1 sb1) /\
         (unchanged_at a2 sa2 sb1) /\
         (unchanged_except a1 sa2 sb2)))
     (ensures (
         (unchanged_at (a1 `L.append` a2) sb1 sb2))) =
-  let precond = !!(disjoint_locations a1 a2) /\
-                 (unchanged_at a1 sa1 sb2) /\
-                 (unchanged_except a2 sa1 sb1) /\
-                 (unchanged_at a2 sa2 sb1) /\
-                 (unchanged_except a1 sa2 sb2) in
+  let a1', a2' = a1 `locations_subtract` a_, a2 `locations_subtract` a_ in
+  let precond = !!(disjoint_locations a1' a2') /\
+                (unchanged_at a_ sb1 sb2) /\
+                (unchanged_at a1 sa1 sb2) /\
+                (unchanged_except a2 sa1 sb1) /\
+                (unchanged_at a2 sa2 sb1) /\
+                (unchanged_except a1 sa2 sb2) in
   let aux1 a :
     Lemma
       (requires (L.mem a a1 /\ precond))
       (ensures (eval_location a sb1 == eval_location a sb2)) =
-    lemma_disjoint_location_from_locations_mem a1 a2 a;
-    assert (!!(disjoint_location_from_locations a a2));
-    assert (eval_location a sb1 == eval_location a sa1);
-    lemma_unchanged_at_mem a1 a sa1 sb2
+    lemma_locations_subtract_mem a a1 a_;
+    lemma_locations_subtract_mem a a2 a_;
+    if L.mem a a_ then (
+      lemma_unchanged_at_mem a_ a sb1 sb2
+    ) else (
+      lemma_disjoint_location_from_locations_mem a1' a2' a;
+      assert (!!(disjoint_location_from_locations a a2'));
+      lemma_disjoint_location_from_locations_subtract a a2 a_;
+      assert (eval_location a sb1 == eval_location a sa1);
+      lemma_unchanged_at_mem a1 a sa1 sb2
+    )
   in
   let aux2 a :
     Lemma
       (requires (L.mem a a2 /\ precond))
       (ensures (eval_location a sb1 == eval_location a sb2)) =
-    lemma_disjoint_locations_symmetric a1 a2;
-    lemma_disjoint_location_from_locations_mem a2 a1 a;
-    assert (!!(disjoint_location_from_locations a a1));
-    assert (eval_location a sb2 == eval_location a sa2);
-    lemma_unchanged_at_mem a2 a sa2 sb1
+    lemma_disjoint_locations_symmetric a1' a2';
+    lemma_locations_subtract_mem a a1 a_;
+    lemma_locations_subtract_mem a a2 a_;
+    if L.mem a a_ then (
+      lemma_unchanged_at_mem a_ a sb1 sb2
+    ) else (
+      lemma_disjoint_location_from_locations_mem a2' a1' a;
+      assert (!!(disjoint_location_from_locations a a1'));
+      lemma_disjoint_location_from_locations_subtract a a1 a_;
+      assert (eval_location a sb2 == eval_location a sa2);
+      lemma_unchanged_at_mem a2 a sa2 sb1
+    )
   in
   let rec aux a1' a1'' a2' a2'' :
     Lemma
@@ -727,6 +784,56 @@ let lemma_both_not_ok (f1 f2:st unit) (rw1 rw2:rw_set) (s:machine_state) :
   lemma_disjoint_implies_unchanged_at rw1.loc_reads rw2.loc_writes s (run f2 s);
   lemma_disjoint_implies_unchanged_at rw2.loc_reads rw1.loc_writes s (run f1 s)
 
+let rec lemma_constant_on_execution_mem
+    (locv:locations_with_values) (f:st unit) (s:machine_state)
+    (l:location{hasEq (location_val_t l)}) (v:location_val_t l) :
+  Lemma
+    (requires (
+        (constant_on_execution locv f s) /\
+        ((run f s).ms_ok) /\
+        ((| l, v |) `L.mem` locv)))
+    (ensures (
+        (eval_location l (run f s) = v))) =
+  match locv with
+  | [_] -> ()
+  | x :: xs ->
+    if x = (| l, v |) then () else (
+      lemma_constant_on_execution_mem xs f s l v
+    )
+
+let lemma_constant_on_execution_stays_constant (f1 f2:st unit) (rw1 rw2:rw_set) (s1 s2:machine_state) :
+  Lemma
+    (requires (
+        (run f1 s1).ms_ok /\ (run f2 s2).ms_ok /\
+        (bounded_effects rw1 f1) /\
+        (bounded_effects rw2 f2) /\
+        (rw1.loc_constant_writes = rw2.loc_constant_writes)))
+    (ensures (
+        unchanged_at (locations_of_locations_with_values rw1.loc_constant_writes)
+          (run f1 s1)
+          (run f2 s2))) =
+  let rec aux c1 c2 :
+    Lemma
+      (requires (
+          (run f1 s1).ms_ok /\ (run f2 s2).ms_ok /\
+          (bounded_effects rw1 f1) /\
+          (bounded_effects rw2 f2) /\
+          (rw1.loc_constant_writes = rw2.loc_constant_writes) /\
+          (c1 `L.append` c2 == rw1.loc_constant_writes)))
+      (ensures (unchanged_at (locations_of_locations_with_values c2) (run f1 s1) (run f2 s2)))
+      (decreases %[c2]) =
+    match c2 with
+    | [] -> ()
+    | y :: ys ->
+      L.append_l_cons y ys c1;
+      L.append_mem c1 c2 y;
+      aux (c1 `L.append` [y]) ys;
+      let (| l, c |) = y in
+      lemma_constant_on_execution_mem rw1.loc_constant_writes f1 s1 l c;
+      lemma_constant_on_execution_mem rw2.loc_constant_writes f2 s2 l c
+  in
+  aux [] rw1.loc_constant_writes
+
 let lemma_commute (f1 f2:st unit) (rw1 rw2:rw_set) (s:machine_state) :
   Lemma
     (requires (
@@ -742,30 +849,36 @@ let lemma_commute (f1 f2:st unit) (rw1 rw2:rw_set) (s:machine_state) :
   if not s12.ms_ok || not s21.ms_ok then (
     lemma_both_not_ok f1 f2 rw1 rw2 s
   ) else (
-    let is1 = run f1 s in
-    let is2 = run f2 s in
-    let is12 = run f2 is1 in
-    let is21 = run f1 is2 in
-    lemma_disjoint_implies_unchanged_at rw1.loc_reads rw2.loc_writes s is2;
-    lemma_disjoint_implies_unchanged_at rw2.loc_reads rw1.loc_writes s is1;
-    assert (unchanged_at rw1.loc_writes is1 is21);
-    assert (unchanged_at rw2.loc_writes is2 is12);
-    assert (unchanged_except rw2.loc_writes s is2);
-    assert (unchanged_except rw1.loc_writes s is1);
-    assert (unchanged_except rw2.loc_writes is1 is12);
-    assert (unchanged_except rw1.loc_writes is2 is21);
-    lemma_unchanged_except_transitive rw1.loc_writes rw2.loc_writes s is1 is12;
-    assert (unchanged_except (rw1.loc_writes `L.append` rw2.loc_writes) s is12);
-    lemma_unchanged_except_transitive rw2.loc_writes rw1.loc_writes s is2 is21;
-    assert (unchanged_except (rw2.loc_writes `L.append` rw1.loc_writes) s is21);
-    lemma_unchanged_except_append_symmetric rw1.loc_writes rw2.loc_writes s is12;
-    lemma_unchanged_except_append_symmetric rw2.loc_writes rw1.loc_writes s is21;
-    lemma_unchanged_except_same_transitive (rw1.loc_writes `L.append` rw2.loc_writes) s is12 is21;
-    lemma_unchanged_at_combine rw1.loc_writes rw2.loc_writes is1 is2 is12 is21;
-    lemma_unchanged_at_and_except (rw1.loc_writes `L.append` rw2.loc_writes) is12 is21;
-    assert (unchanged_except [] is12 is21);
+    let s1 = run f1 s in
+    let s2 = run f2 s in
+    let r1, w1, c1 = rw1.loc_reads, rw1.loc_writes, rw1.loc_constant_writes in
+    let r2, w2, c2 = rw2.loc_reads, rw2.loc_writes, rw1.loc_constant_writes in
+    let dw1 = w1 `locations_subtract` (locations_of_locations_with_values c1) in
+    let dw2 = w2 `locations_subtract` (locations_of_locations_with_values c2) in
+    assert (locations_of_locations_with_values c1 = locations_of_locations_with_values c2);
+    let const = locations_of_locations_with_values c1 in
+    assert (s12 == run f2 s1 /\ s21 == run f1 s2);
+    lemma_disjoint_implies_unchanged_at r1 w2 s s2;
+    lemma_disjoint_implies_unchanged_at r2 w1 s s1;
+    assert (unchanged_at w1 s1 s21);
+    assert (unchanged_at w2 s2 s12);
+    assert (unchanged_except w2 s s2);
+    assert (unchanged_except w1 s s1);
+    assert (unchanged_except w2 s1 s12);
+    assert (unchanged_except w1 s2 s21);
+    lemma_unchanged_except_transitive w1 w2 s s1 s12;
+    assert (unchanged_except (w1 `L.append` w2) s s12);
+    lemma_unchanged_except_transitive w2 w1 s s2 s21;
+    assert (unchanged_except (w2 `L.append` w1) s s21);
+    lemma_unchanged_except_append_symmetric w1 w2 s s12;
+    lemma_unchanged_except_append_symmetric w2 w1 s s21;
+    lemma_unchanged_except_same_transitive (w1 `L.append` w2) s s12 s21;
+    lemma_constant_on_execution_stays_constant f2 f1 rw2 rw1 s1 s2;
+    lemma_unchanged_at_combine w1 w2 const s1 s2 s12 s21;
+    lemma_unchanged_at_and_except (w1 `L.append` w2) s12 s21;
+    assert (unchanged_except [] s12 s21);
     assert (s21.ms_ok = s12.ms_ok);
-    lemma_equiv_states_when_except_none is12 is21 s12.ms_ok;
+    lemma_equiv_states_when_except_none s12 s21 s12.ms_ok;
     assert (equiv_states (run2 f1 f2 s) (run2 f2 f1 s))
   )
 
